\documentclass[noinstructornotes]{ximera}
%handout:  for handout version with no solutions or instructor notes
%handout,instructornotes:  for instructor version with just problems and notes, no solutions
%noinstructornotes:  shows only problem and solutions

%% handout
%% space
%% newpage
%% numbers
%% nooutcomes

%I added the commands here so that I would't have to keep looking them up
%\newcommand{\RR}{\mathbb R}
%\renewcommand{\d}{\,d}
%\newcommand{\dd}[2][]{\frac{d #1}{d #2}}
%\renewcommand{\l}{\ell}
%\newcommand{\ddx}{\frac{d}{dx}}
%\everymath{\displaystyle}
%\newcommand{\dfn}{\textbf}
%\newcommand{\eval}[1]{\bigg[ #1 \bigg]}

%\begin{image}
%\includegraphics[trim= 170 420 250 180]{Figure1.pdf}
%\end{image}

%add a ``.'' below when used in a specific directory.
\input{../preamble.tex} %% we can turn off input when making a master document
\usepackage{fullpage}

\title{Recitation \# 7: Exponential Models and Integration By Parts}  

\begin{document}
\begin{abstract}		\end{abstract}
\maketitle



\begin{comment}
\section{Warm up:}

	\begin{freeResponse}
	
	\end{freeResponse}
	
\begin{instructorNotes}

\end{instructorNotes}
\end{comment}







\section{Group work:}



%problem 1
\begin{problem}
Vitameatavegamin is a strange substance that comes in two forms.  
V-I decays at a linear rate, while V-II decays at an exponential rate.  
Both have the property that $10$ ounces will decrease to $7$ ounces in $6$ hours.  
For each of V-I and V-II, answer the following:
	\begin{enumerate}
	
	\item  If we started with $80$ ounces, how much will there be $6$ hours later?
	\begin{freeResponse}
	\dfn{V-I:}  Recall that in the linear decay model
		\[
		y(t) = -k \cdot t + y_0
		\]
	where $k$ denotes the rate of decay and $y_0$ is the initial amount.  
	We are given that $y_0 = 80oz$.  
	Clearly, we also have that
		\[
		y'(t) = -k.
		\]
	In the linear decay model, the rate of decay does not depend on the initial amount.  
	So from the given information, we have that
		\[
		-k = \frac{10oz - 7oz}{0hr - 6hr} = - \frac{1}{2}.  
		\]
	Thus, $y(t) = - \frac{1}{2} t + 80$, and therefore
		\[
		y(6) = - \frac{1}{2} (6) + 80 = 77 oz.
		\]
		
	\vskip 10pt	
		
	\dfn{V-II:}  Recall that in the exponential decay model
		\[
		y(t) = y_0 \cdot e^{-k \cdot t}
		\]
	where again $y_0 = 80oz$ is the initial amount.  
	Also notice that
		\begin{align*}
		y'(t) &= -k y_0 e^{-kt}  \\
		&= -k y(t)  \\
		\Longrightarrow &\qquad y'(0) = -k y_0.
		\end{align*}
	
	It is given that it takes $6$ hours for $10$ ounces to decrease to $7$ ounces.  
	In other words, it takes $6$ hours for $70\%$ of the substance to remain.
	So we have that
		\begin{align*}
		y(6) &= \frac{7}{10} y_0  \\
		&\Longrightarrow  \qquad  y_0 e^{-k \cdot 6} = \frac{7}{10} y_0  \\
		&\Longrightarrow  \qquad  e^{-6k} = \frac{7}{10}  \\
		&\Longrightarrow  \qquad -6k = \ln \left(\frac{7}{10} \right) = - \ln \left( \frac{10}{7} \right)  \\
		&\Longrightarrow  \qquad  k = \frac{1}{6} \ln \left( \frac{10}{7} \right).
		\end{align*}
	Thus,
		\begin{align*}
		y(6) &= 80 e^{- \frac{1}{6} \ln \left( \frac{10}{7} \right) \cdot 6}  \\
		&= 80 e^{- \ln \left( \frac{10}{7} \right)}  \\
		&= 80 \cdot \frac{7}{10} = 56oz.
		\end{align*}
	\end{freeResponse}
	
	
	
	\item  How long will it take to decrease from $15$ ounces to $7.5$ ounces?
	\begin{freeResponse}
	\dfn{V-I:}  Recall from above that $k = \frac{1}{2}$.  
	Then since $y_0$ is now $15$, we have that
		\[
		y(t) = - \frac{1}{2} t + 15.
		\]
	We want to find $t$ such that $y(t) = 7.5$.  
	So we solve
		\begin{align*}
		7.5 &= - \frac{1}{2} t + 15  \\
		- \frac{15}{2} &= - \frac{1}{2} t  \\
		t &= 15 \text{ hours}.
		\end{align*}
		
	\vskip 10pt
	
	\dfn{V-II:}  Again, since $y_0$ is now $15$, we know from above that
		\[
		y(t) = 15 e^{- \frac{1}{6} \ln \left( \frac{10}{7} \right) \cdot t}.
		\]
	We want to find $t$ such that $y(t) = 7.5 = \frac{15}{2}$.  So we solve
		\begin{align*}
		\frac{15}{2} &= 15 e^{- \frac{1}{6} \ln \left( \frac{10}{7} \right) \cdot t}  \\
		\frac{1}{2} &= e^{- \frac{1}{6} \ln \left( \frac{10}{7} \right) \cdot t}  \\
		\ln \left( \frac{1}{2} \right) &= - \frac{1}{6} \ln \left( \frac{10}{7} \right) \cdot t  \\
		\ln \left( \frac{10}{7} \right) t &= - 6 \ln \left( \frac{1}{2} \right) = 6 \ln 2  \\
		t &= \frac{6 \ln 2}{\ln \left( \frac{10}{7} \right) } \text{ hours}.
		\end{align*}
	\end{freeResponse}
	
	\end{enumerate}
	
\end{problem}

\begin{instructorNotes}
The issue is to compare and contrast linear and exponential decay.  
To solve, it is implicit to find the slope (I) and $k$ (II) first before proceeding (this may need a prompt).
\end{instructorNotes}



%problem 2
\begin{problem}
Evaluate the following integrals
	\begin{enumerate}
	
	\item  $\int_1^3 x^2 5^x \d x$
	\begin{freeResponse}
	We proceed via integration by parts.  Let 
		{\color{red}
		\[
		u = x^2, \qquad \d v = 5^x \d x
		\]
		}
	so that
		{\color{red}
		\[
		\d u = 2x \d x, \qquad v = \frac{5^x}{\ln 5} .
		\]
		}
	Recall the formula for integration by parts is
		\[
		\int_a^b u \d v = \eval{uv}_a^b - \int_a^b v \d u.
		\]
	So we substitute
		\begin{align*}
		\int_1^3 x^2 5^x \d x &= \eval{\frac{x^2 5^x}{\ln(5)}}_1^3 - \int_1^3 2x \frac{5^x}{\ln(5)} \d x  \\
		&= \frac{1}{\ln(5)} \left( 9 \cdot 5^3 - 5 \right) - \frac{2}{\ln(5)} \int_1^3 x 5^x \d x.
		\end{align*}
	For the remaining integral we again use integration by parts:
		{\color{red}
		\[
		u = x, \qquad \d v = 5^x  
		\]
		\[
		\d u = \d x, \qquad v = \frac{5^x}{\ln(5)}.
		\]
		}
	Thus,
		\begin{align*}
		&\frac{1}{\ln(5)} \left( 9 \cdot 5^3 - 5 \right) - \frac{2}{\ln(5)} \int_1^3 x 5^x \d x \\
		&= \frac{5}{\ln(5)} (225 - 1) - \frac{2}{\ln(5)} \left( \eval{\frac{x5^x}{\ln(5)}}_1^3 - \int_1^3 \frac{5^x}{\ln(5)} \d x \right)  \\
		&= \frac{1120}{\ln(5)} - \frac{2}{\ln^2(5)} \left( (3 \cdot 5^3 - 5) - \eval{\frac{5^x}{\ln(5)}}_1^3 \right)  \\
		&= \frac{1}{\ln(5)} \left( 1120 - \frac{740}{\ln(5)} + \frac{248}{\ln^2(5)} \right).
		\end{align*}
	\end{freeResponse}
	
	

	\item $\int \arcsin(x) \d x$
	\begin{freeResponse}
	We do not know how to integrate $\arcsin(x)$, but we do know how to differentiate it, so we will use integration by parts. 
		{\color{red}
		\[
		u = arcsin(x)	\qquad	\d v =  \d x
		\]
		\[
		\d u = \frac{1}{\sqrt{1-x^2}} \d x	\qquad	v = x
		\]}
	This gives us
	\begin{align*}
	\int \arcsin(x) \d x &= x\arcsin(x) - \int \frac{x \d x}{\sqrt{1-x^2}} \\
	& \\
	u &= 1-x^2 \\
	\d u &= -2x \d x \\
	-\frac{1}{2}\d u &= \d x \\
	& \\
	\int \frac{x \d x}{\sqrt{1-x^2}} &= \int \frac{-\d u}{2\sqrt{u}}\\
	&= -\frac{1}{2} \int u^{-\frac{1}{2}} \d u \\
	&= -\frac{1}{2} \cdot 2u^{\frac{1}{2}} +C \\
	&= - \sqrt{1-x^2} +C
	& \\
	\int \arcsin(x) \d x &= x\arcsin(x) - \int \frac{x \d x}{\sqrt{1-x^2}} \\
	&=x\arcsin(x) - \left(  - \sqrt{1-x^2} \right) +C \\
	&=x\arcsin(x) + \sqrt{1-x^2} +C 
	\end{align*}
	
	\end{freeResponse}
	
	
	\item  $\int x^{\frac{5}{3}} (\ln x)^2 \d x$
	\begin{freeResponse}
	We begin with the substitution
		{\color{red}
		\[
		w = \ln x 	\qquad	\Longrightarrow	\qquad	\d w = \frac{1}{x} \d x, \quad  x = e^w.
		\]}
	Then
		\begin{align*}
		\int x^{\frac{5}{3}} (\ln x)^2 \d x 
		&= \int x^{\frac{8}{3}} (\ln x)^2 \cdot \frac{1}{x} \d x  \\
		&= \int (e^w)^{\frac{8}{3}} w^2 \d w  \\
		&= \int w^2 e^{\frac{8}{3} w} \d w.
		\end{align*}
	We now use integration by parts, with
		{\color{red}
		\[
		u = w^2	\qquad	\d v = e^{\frac{8}{3} w} \d w
		\]
		\[
		\d u = 2w \d w	\qquad	v = \frac{3}{8} e^{\frac{8}{3} w}.
		\]}
	This gives us
		\begin{align*}
		\int x^{\frac{5}{3}} (\ln x)^2 \d x
		&= \frac{3}{8} w^2 e^{\frac{8}{3} w} - \int \frac{3}{8} (2w) e^{\frac{8}{3} w} \d w  \\
		&= \frac{3}{8} w^2 e^{\frac{8}{3} w} - \frac{3}{4} \int w e^{\frac{8}{3} w} \d w.
		\end{align*}
	We apply integration by parts one last time with
	{\color{red}
		\[
		u = w		\qquad	\d v = e^{\frac{8}{3} w} \d w
		\]
		\[
		\d u = \d w	\qquad	v = \frac{3}{8} e^{\frac{8}{3} w}
		\]}
	which yields
		\begin{align*}
		\int x^{\frac{5}{3}} (\ln x)^2 \d x
		&= \frac{3}{8}w^2 e^{\frac{8}{3} w} - \frac{3}{4} \left( \frac{3}{8} w e^{\frac{8}{3} w} - \frac{3}{8} \int e^{\frac{8}{3} w} \d w \right) \\
		&= \frac{3}{8} w^2 e^{\frac{8}{3} w} - \frac{9}{32} w e^{\frac{8}{3} w} + \frac{27}{256} e^{\frac{8}{3} w} + C  \\
		&= \frac{3}{8} e^{\frac{8}{3} \ln x} \left( (\ln x)^2 - \frac{3}{4} \ln x + \frac{9}{32} \right) + C  \\
		&= \frac{3}{8} x^{\frac{8}{3}} \left( (\ln x)^2 - \frac{3}{4} \ln x + \frac{9}{32} \right) + C.
		\end{align*}
	\end{freeResponse}
	
	\end{enumerate}
	
\end{problem}

\begin{instructorNotes}
All three parts involve standard strategies learned in the online lessons.  
For each, split the problems between the groups.  
Then discuss each problem as a class, getting input from the group(s) that worked on that problem.
\end{instructorNotes}






%problem 3
\begin{problem}

Evaluate the following integral

	$\int \sin(3x) e^{7x} \d x$
	\begin{freeResponse}
	We begin by letting $I = \int \sin(3x) e^{7x} \d x$.  
	We then use integration by parts with
		{\color{red}
		\[
		u = e^{7x} \qquad \d v = \sin(3x) \d x
		\]
		\[
		\d u = 7e^{7x} \d x \qquad v = -\frac{1}{3} \cos(3x).
		\]
		}
	Then
		\begin{align*}
		\int \sin(3x) e^{7x} \d x = I
		&= -\frac{1}{3} e^{7x} \cos(3x) - \int -\frac{1}{3} (7e^{7x}) \cos(3x) \d x  \\
		I &= -\frac{1}{3} e^{7x} \cos(3x) + \frac{7}{3} \int e^{7x} \cos(3x) \d x.
		\end{align*}
	We then apply integration by parts again, this time with
		{\color{red}
		\[
		u = e^{7x} 		\qquad	\d v = \cos(3x) \d x
		\]
		\[
		\d u = 7e^{7x} \d x 	\qquad	v = \frac{1}{3} \sin(3x).
		\]
		}
	This gives us
		\begin{align*}
		I &= -\frac{1}{3} e^{7x} \cos(3x) + \frac{7}{3} \left[ \frac{1}{3} e^{7x} \sin(3x) - \int \frac{1}{3} (7e^{7x}) \sin(3x) \d x \right]  \\
		I &= -\frac{1}{3} e^{7x} \cos(3x) + \frac{7}{9} e^{7x} \sin(3x) - \frac{49}{9} \int e^{7x} \sin(3x) \d x  \\
		I &= -\frac{1}{3} e^{7x} \cos(3x) + \frac{7}{9} e^{7x} \sin(3x) - \frac{49}{9} I  \\
		\frac{58}{9} I &= -\frac{1}{3} e^{7x} \cos(3x) + \frac{7}{9} e^{7x} \sin(3x)  \\
		I &= \frac{9}{58} \left( -\frac{1}{3} e^{7x} \cos(3x) + \frac{7}{9} e^{7x} \sin(3x) \right) + C.
		\end{align*}
	\end{freeResponse}

\end{problem}





%problem 4
\begin{problem}
Evaluate the following integrals
	\begin{enumerate}
	
	\item  $\int x^5 \cos \left( x^3 \right) \d x$
	\begin{freeResponse}
	We begin with the substitution
		{\color{red}
		\[
		w = x^3 	\qquad	\Longrightarrow	\qquad	\d w = 3x^2 \d x, 	\quad	\frac{1}{3} \d w = x^2 \d x.
		\]
		}
	Then,
		\begin{align*}
		\int x^5 \cos \left( x^3 \right) \d x 
		&= \int x^3 \cos \left( x^3 \right) \cdot x^2 \d x  \\
		&= \int w \cos(w) \cdot \frac{1}{3} \d w  \\
		&= \frac{1}{3} \int w \cos(w) \d w.
		\end{align*}
	We then use integration by parts, with
		{\color{red}
		\[
		u = w 		\qquad	\d v = \cos(w) \d w
		\]
		\[
		\d u = \d w 	\qquad	v = \sin(w)
		\]
		}
	which yields
		\begin{align*}
		\int x^5 \cos \left( x^3 \right) \d x 
		&= \frac{1}{3} \left( w \sin(w) - \int \sin(w) \d w \right)  \\
		&= \frac{1}{3} \left( w \sin(w) + \cos(w) \right) + C  \\
		&= \frac{1}{3} \left( x^3 \sin \left( x^3 \right) + \cos \left( x^3 \right) \right) + C.  
		\end{align*}
	\end{freeResponse}
	
	
	
	\item  $\int \cos \left( \sqrt{x} \right) \d x$
	\begin{freeResponse}
	We begin with the subsitution
		{\color{red}
		\[
		w = \sqrt{x} 	\qquad	\Longrightarrow	\qquad	\d w = \frac{1}{2\sqrt{w}} \d w, \quad	2 \d w = \frac{1}{\sqrt{x}} \d w.
		\]
		}
	Then
		\begin{align*}
		\int \cos \left( \sqrt{x} \right) \d x 
		&= \int \cos \left( \sqrt{x} \right) \cdot \frac{\sqrt{x}}{\sqrt{x}} \d x  \\
		&= 2 \int w \cos(w) \d w  \\
		&= 2 (w \sin(w) + \cos(w)) + C 	\qquad	{\color{red}\text{From part (a)}}  \\
		&=2 \left( \sqrt{x} \sin \left( \sqrt{x} \right) + \cos \left( \sqrt{x} \right) \right) + C.
		\end{align*}
	\end{freeResponse}
	
	
	
	\item  $\int x \cos x \sin x \d x$
	\begin{freeResponse}
	First, recall that
		{\color{red}
		\[
		\sin(2x) = 2 \sin x \cos x 	\qquad	\Longrightarrow	\qquad	\sin x \cos x = \frac{1}{2} \sin(2x).
		\]
		}
	So we can rewrite the given integral as
		\[
		\int x \cos x \sin x \d x = \frac{1}{2} \int x \sin(2x) \d x.
		\]
	Now we use integration by parts with
		{\color{red}
		\[
		u = x 		\qquad	\d v = \sin(2x) \d x
		\]
		\[
		\d u = \d x 	\qquad	v = - \frac{1}{2} \cos(2x).
		\]
		}
	This gives us that
		\begin{align*}
		\frac{1}{2} \int x \sin(2x) \d x
		&= \frac{1}{2} \left( - \frac{1}{2} x \cos(2x) - \int -\frac{1}{2} \cos(2x) \d x \right)  \\
		&= \frac{1}{4} \left( -x \cos(2x) + \frac{1}{2} \sin(2x) \right) + C.
		\end{align*}
	\end{freeResponse}
	
	\end{enumerate}
	
\end{problem}

\begin{instructorNotes}
For this problem, you might just lead a whole class discussion - hopefully soliciting ideas from the students (on their own or with hints).  
You might want to note that some of the problems may be approached in different ways.  
For example, one could begin part (a) with either the substitution $u=x^3$ or by parts with $u=x^3, \d v = x^2 \cos(x^3)$.
\end{instructorNotes}













								
				
				
	














\end{document} 


















