\documentclass[noinstructornotes]{ximera}
%handout:  for handout version with no solutions or instructor notes
%handout,instructornotes:  for instructor version with just problems and notes, no solutions
%noinstructornotes:  shows only problem and solutions

%% handout
%% space
%% newpage
%% numbers
%% nooutcomes

%I added the commands here so that I would't have to keep looking them up
%\newcommand{\RR}{\mathbb R}
%\renewcommand{\d}{\,d}
%\newcommand{\dd}[2][]{\frac{d #1}{d #2}}
%\renewcommand{\l}{\ell}
%\newcommand{\ddx}{\frac{d}{dx}}
%\everymath{\displaystyle}
%\newcommand{\dfn}{\textbf}
%\newcommand{\eval}[1]{\bigg[ #1 \bigg]}

%\begin{image}
%\includegraphics[trim= 170 420 250 180]{Figure1.pdf}
%\end{image}

%add a ``.'' below when used in a specific directory.
\input{../preamble.tex} %% we can turn off input when making a master document

\title{Basic approaches}  

\begin{document}
\begin{abstract}		\end{abstract}
\maketitle



\begin{comment}
\section{Warm up:}

	\begin{freeResponse}
	
	\end{freeResponse}
	
\begin{instructorNotes}

\end{instructorNotes}
\end{comment}







\section{Group work:}



%problem 1
\begin{problem}
Evaluate
	\[
	\int \frac{5x^3 - 6x + 2}{x-5} \d x.
	\]
	\begin{freeResponse}
	When integrating a rational function (i.e., a fraction of polynomials) where the degree of the numerator is greater than or equal to the degree of the denominator, we need to use long division to simplify the expression.  
	
	\begin{image}
	\includegraphics[trim= 170 220 250 250, scale=0.7]{Figure7-1-1.pdf}
	\end{image}
	
	So
		\[
		\frac{5x^3 - 6x + 2}{x-5} = 5x^2 + 25x + 119 + \frac{597}{x-5}
		\]
	and therefore
		\begin{align*}
		\int \frac{5x^3 - 6x + 2}{x-5} \d x &= \int \left( 5x^2 + 25x + 119 + \frac{597}{x-5} \right) \d x  \\
		&= \frac{5}{3} x^3 + \frac{25}{2} x^2 + 119x + 597 \int \frac{1}{x-5} \d x.
		\end{align*}
	To evaluate
		\[
		\int \frac{1}{x-5} \d x
		\]
	we technically should perform a substitution.  
	But since $\ddx (x-5) = 1$, we can treat $x-5$ as a variable during integration.  
	Thus
		\[
		\int \frac{1}{x-5} \d x = \ln |x-5|
		\]
	and therefore
		\[
		\int \frac{5x^3 - 6x + 2}{x-5} \d x = \frac{5}{3} x^3 + \frac{25}{2} x^2 + 119x + 597 \ln |x-5| + C.
		\]
	\end{freeResponse}
	
\end{problem}

\begin{instructorNotes}
Each of problems \#1 through \#4 presents a different aspect that is covered in Section 7.1.  
This problem (\# 1) requires long division.  
\end{instructorNotes}







%problem 2
\begin{problem}
Evaluate
	\[
	\int \frac{5}{3^{2x} + 3^{-2x}} \d x.
	\]
	\begin{freeResponse}
		\begin{align*}
		\int \frac{5}{3^{2x} + 3^{-2x}} \d x &= \int \frac{5}{3^{2x} + 3^{-2x}} \cdot \frac{3^{2x}}{3^{2x}} \d x  \\
		&= \int \frac{5 \cdot 3^{2x}}{\left( 3^{2x} \right)^2 + 1} \d x .
		\end{align*}
	Now, let 
		\[
		u = 3^{2x}.
		\]  
	Then 
		\[
		\d u = 2 \cdot 3^{2x} \cdot \ln (3) \d x
		\]
	and so
		\[
		\d x = \frac{1}{2 \cdot 3^{2x} \cdot \ln (3)} \d u.
		\]
	Thus
		\begin{align*}
		\int \frac{5}{3^{2x} + 3^{-2x}} \d x &= \int \frac{5}{u^2 + 1} \cdot \frac{1}{2\ln(3)} \d u  \\
		&= \frac{5}{2\ln(3)} \arctan(u) + C  \\
		&= \frac{5}{2\ln(3)} \arctan \left( 3^{2x} \right) + C.
		\end{align*}
	\end{freeResponse}
		
\end{problem}

\begin{instructorNotes}
Students are likely to have forgotten $\ddx \left( C^x \right)$ for $C \neq e$.
\end{instructorNotes}







%problem 3
\begin{problem}
Evaluate the following integrals
	\begin{enumerate}
	
	\item  $\int \frac{\cos x}{1 + \sin x} \d x$
	\begin{freeResponse}
	Let $u=1+\sin x$.  Then $\d u = \cos x \d x$, and so
		\begin{align*}
		\int \frac{\cos x}{1 + \sin x} \d x &= \int \frac{1}{u} \d u  \\
		&= \ln|u| + C  \\
		&= \ln (1 + \sin(x) ) + C.
		\end{align*}
	\end{freeResponse}
	
	
	
	\item  $ \int \frac{1}{\sin x - 1} \d x$
	\begin{freeResponse}
		\begin{align*}
		\int \frac{1}{\sin x - 1} \d x &= \int \frac{1}{\sin x - 1} \cdot \frac{\sin x + 1}{\sin x + 1} \d x  \qquad  {\color{red}\text{since } \frac{\sin x + 1}{\sin x + 1} = 1}\\
		&= \int \frac{\sin x + 1}{\sin^2 x - 1} \d x  \\
		&= \int \frac{\sin x + 1}{-\cos^2 x} \d x		\qquad	{\color{red}\text{since } \cos^2 x + \sin^2 x = 1}  \\
		&= \int \frac{-\sin x}{\cos^2 x} \d x - \int \frac{1}{\cos^2 x} \d x.
		\end{align*}
	Now we split up and compute these two integrals separately.
		\begin{align*}
		\int \frac{-\sin x}{\cos x} \d x &= \int \frac{1}{u^2} \d u	\qquad	{\color{red} \text{where } u = \cos x, \d u = - \sin x \d x}  \\
		&= - \frac{1}{u} + C = \frac{-1}{\cos x} + C.
		\end{align*}
	Also,
		\[
		\int \frac{1}{\cos^2 x} \d x = \int \sec^2 x \d x = \tan x + C.
		\]
	So, we finally have that
		\[
		\int \frac{1}{\sin x - 1} \d x = \frac{-1}{\cos x} - \tan x + C.
		\]
	\end{freeResponse}
	
	\end{enumerate}

\end{problem}

\begin{instructorNotes}
The two integrals in this problem look similar, but they require very different strategies in order to rewrite them as ``basic" integrals.
\end{instructorNotes}







%problem 4
\begin{problem}
Evaluate the following integrals
	\begin{enumerate}
	
	\item  $ \int \frac{13}{\sqrt{12x - x^2 - 20}} \d x$
	\begin{freeResponse}
	First notice that by completing the square, we have that
		\begin{align*}
		12x - x^2 - 20 &= -(x^2 - 12x) - 20  \\
		&= -(x^2 - 12x + {\color{red}36}) - 20 + {\color{red}36}  \\
		&= 16 - (x-6)^2  \\
		&= 16 \left( 1 - \frac{(x-6)^2}{16} \right)  \\
		&= 16 \left( 1 - \left( \frac{x-6}{4} \right)^2 \right).
		\end{align*}
	Then
		\begin{align*}
		\int \frac{13}{\sqrt{12x - x^2 - 20}} \d x &= \int \frac{13}{\sqrt{16 \left( 1 - \left( \frac{x-6}{4} \right)^2 \right)}} \d x  \\
		&= \frac{13}{4} \int \frac{1}{\sqrt{1 - \left( \frac{x-6}{4} \right)^2}} \d x.
		\end{align*}
	
	Let
		\[
		u = \frac{x-6}{4} = \frac{1}{4} (x-6).
		\]
	Then
		\[
		\d u = \frac{1}{4} \d x		\qquad	\Longrightarrow		\qquad	4 \d u = \d x.
		\]
	Finally, we have that
		\begin{align*}
		\int \frac{13}{\sqrt{12x - x^2 - 20}} \d x &= 13 \int \frac{1}{\sqrt{1-u^2}} \d u  \\
		&= 13 \arcsin(u) + C  \\
		&= 13 \arcsin \left( \frac{x-6}{4} \right) + C.
		\end{align*}
	\end{freeResponse}
	
	
	
	\item  $\int \frac{13x^3}{\sqrt{12x^6 - x^8 - 20x^4}} \d x$
	\begin{freeResponse}
		\begin{align*}
		\int \frac{13x^3}{\sqrt{12x^6 - x^8 - 20x^4}} \d x &= \int \frac{13x^3}{\sqrt{x^4} \cdot \sqrt{12x^2-x^4-20}} \d x  \\
		&= \int \frac{13x}{\sqrt{12x^2-x^4-20}} \d x  \\
		&= \frac{1}{2} \int \frac{13}{\sqrt{12u-u^2-20}} \d u	\qquad	{\color{red} \text{Let }u=x^2, \d u = 2 x \d x }  \\
		&= \frac{1}{2} \left( 13 \arcsin \left( \frac{u-6}{4} \right) \right) + C	\qquad	{\color{red}\text{from part (a)}}  \\
		&= \frac{13}{2} \arcsin \left( \frac{x^2 - 6}{4} \right) + C.
		\end{align*}
	\end{freeResponse}
	
	
	
	\item  $\int \frac{13e^{4x}}{\sqrt{ 12e^{6x} - e^{8x} - 20e^{4x} }} \d x$
	\begin{freeResponse}
		\begin{align*}
		\int \frac{13e^{4x}}{\sqrt{ 12e^{6x} - e^{8x} - 20e^{4x} }} \d x &= \int \frac{13e^{4x}}{\sqrt{e^{4x}} \cdot \sqrt{12e^{2x} - e^{4x} - 20}} \d x  \\
		&= \int \frac{13e^{2x}}{\sqrt{12e^{2x} - e^{4x} - 20}} \d x  \\
		&= \frac{1}{2} \int \frac{13}{\sqrt{12u - u^2 - 20}} \d u		\qquad	{\color{red} \text{where } u=e^{2x}, \d u = 2e^{2x} \d x}  \\
		&= \frac{1}{2} \left( 13 \arcsin \left( \frac{u-6}{4} \right) \right) + C	\qquad 	{\color{red}\text{from part (a)}}  \\
		&= \frac{13}{2} \arcsin \left( \frac{e^{2x}-6}{4} \right) + C.
		\end{align*}
	\end{freeResponse}
	
	\end{enumerate}

\end{problem}

\begin{instructorNotes}
Part (a) of this problem involves completing the square.  
Parts (b) and (c) both require you to factor out a common factor, as well as substitute, to get the same integral as in part (a).  
You may want to do part (a) as a whole class, and then split parts (b) and (c) between the groups.  
Then let them present the substitution which returns part (a).  
\end{instructorNotes}
















	
	
	
	
	
	
	
	
	

	










								
				
				
	














\end{document} 


















